theories/DMin/synNMOfeOpenSemTypes.v
@@ -20,19 +20,19 @@ Section openSemanticSyntax.
   Context {Σ : gFunctors}. (* Look ma', no requirements! *)
   (* Here, we put the later around the whole function, as an experiment.
      This *)
-  Definition semVls: cFunctor := (synCF (▶ ((varC -n> ∙) -n> ∙ -n> iProp Σ)) vls)%CF.
+  Definition semVls: cFunctor := (synCF ((var -c> ▶ ∙) -n> ▶ ∙ -n> iProp Σ) vls)%CF.
   Import cofe_solver.
 
   Definition semVls_result:
     solution semVls := solver.result _.
   Definition iPreVl: ofeT := semVls_result.
 
-  Definition preD := (varC -n> iPreVl) -n> iPreVl -n> iProp Σ.
-  Definition iSyn s : ofeT := synC (laterC preD) s.
+  Definition preD := (var -c> laterC iPreVl) -n> laterC iPreVl -n> iProp Σ.
+  Definition iSyn s : ofeT := synC preD s.
 
   Notation "'vl'" := (iSyn vls).
   Notation "'tm'" := (iSyn tms).
-  Notation D := ((varC -n> vl) -n> vl -n> iProp Σ).
+  Notation D := ((var -c> vl) -n> vl -n> iProp Σ).
 
   (*
   Inspired from code in
@@ -45,36 +45,69 @@ Section openSemanticSyntax.
   Proof. apply solution_unfold_fold. Qed.
   Lemma iSyn_unfold_fold (v : iPreVl) : iSyn_unfold (iSyn_fold v) ≡ v.
   Proof. apply solution_fold_unfold. Qed.
+
+  Program Definition iSyn_unfold' : vl -n> laterC iPreVl :=
+    CofeMor Next ◎ iSyn_unfold.
+  Program Definition iSyn_fold' : laterC iPreVl → vl :=
+    iSyn_fold ∘ later_car.
+  Global Arguments iSyn_unfold': simpl never.
+  Global Arguments iSyn_fold': simpl never.
+  Instance iSyn_fold'_anti_contractive n :
+    Proper (dist n ==> dist_later n) iSyn_fold'.
+  Proof. move :n =>[|n]; rewrite /iSyn_fold' => *??? //=. by f_equiv. Qed.
+  Lemma iSyn_fold_unfold' (v : vl) : iSyn_fold' (iSyn_unfold' v) ≡ v.
+  Proof. apply solution_unfold_fold. Qed.
+  Lemma iSyn_unfold_fold' (v : laterC iPreVl) : iSyn_unfold' (iSyn_fold' v) ≡ v.
+  Proof. apply solution_fold_unfold. Qed.
+
   (* Semantic types! *)
 
   (* Check that values contain terms. *)
   Definition _test (v: vl) (t: tm) : iProp Σ :=
     (∃ Φ t, v ≡ vpack Φ t)%I.
 
-  Program Definition unpack: laterC preD -n> D :=
-    λne '(Next Φ) ρ v, (▷ Φ (λne x, (iSyn_unfold (ρ x))) (iSyn_unfold v))%I.
+  Program Definition unpack: preD -n> D :=
+    λne Φ ρ v, Φ (iSyn_unfold' ∘ ρ) (iSyn_unfold' v).
   (* Body copy-pasted from somewhere in Iris (but had simpl, not cbn). *)
   Ltac solve_proper_cbn := solve_proper_core ltac:(fun _ => first [ intros ?; progress simpl | f_equiv ]).
-  Solve All Obligations with solve_contractive || solve_proper_cbn.
+  Ltac solve_contractive_cbn := solve_proper_core ltac:(fun _ => first [ intros ?; progress simpl | f_contractive | f_equiv ]).
+  Ltac solve_proper_ho_core tac :=
+  solve [repeat intro; cbn; repeat tac (); cbn in *;
+  repeat match goal with H : _ ≡{_}≡ _|- _ => apply H end].
+  Ltac solve_proper_ho := solve_proper_ho_core ltac:(fun _ => first [intros ?; progress simpl | f_equiv]).
+  Ltac solve_contractive_ho := solve_proper_ho_core ltac:(fun _ => first [intros ?; progress simpl | f_contractive | f_equiv]).
+
+  Solve All Obligations with solve_proper_ho.
 
   (** Note that here we get an extra later when we *pack*
       predicates (so that we can pass them to vpack). *)
-  Program Definition pack: D -n> laterC preD :=
-    λne Φ, Next (λne ρ v, Φ (λne x, iSyn_fold (ρ x)) (iSyn_fold v))%I.
-  Solve All Obligations with solve_contractive || solve_proper_cbn.
-
-  Lemma unpack_pack Φ ρ v: unpack (pack Φ) ρ v ≡ (▷ Φ ρ v)%I.
-  Proof.
-    (* rewrite /= iSyn_fold_unfold. (repeat f_equiv) => ? /=. *)
-    (* exact: iSyn_fold_unfold. *)
-    solve_proper_core
-      ltac:(fun _ => first [ rewrite iSyn_fold_unfold | intros ?; progress simpl | f_equiv ]).
+  Program Definition pack: D -n> preD :=
+    λne Φ ρ v, (▷ Φ (λne x, iSyn_fold' (ρ x)) (iSyn_fold' v))%I.
+  Solve All Obligations with rewrite /iSyn_fold'; (solve_contractive || solve_proper_cbn || solve_contractive_ho || solve_proper_ho).
+  Next Obligation.
+    rewrite /iSyn_fold' =>*?? H[?]/=.
+    f_contractive; repeat f_equiv; move=>?/=.
+    f_equiv. apply H.
   Qed.
-  Program Definition later_preD : preD -n> preD := (λne Φ ρ v, ▷ Φ ρ v)%I.
+  Solve All Obligations with rewrite /iSyn_fold'; solve_contractive || solve_proper_cbn || solve_contractive_ho || solve_proper_ho.
+
+  Program Definition later_pred {A B: ofeT}:
+    (A -n> B -n> iProp Σ) -n> (A -n> B -n> iProp Σ) :=
+    (λne Φ ρ v, ▷ Φ ρ v)%I.
   Solve All Obligations with solve_proper.
 
-  Lemma pack_unpack (Φ: preD):
-    pack (unpack (Next Φ)) ≡ Next (later_preD Φ).
+  Lemma unpack_pack Φ: unpack (pack Φ) ≡ later_pred Φ.
+  Proof.
+    move=>??/=; rewrite iSyn_fold_unfold'.
+    (repeat f_equiv) =>?/=. by rewrite /= iSyn_fold_unfold'.
+
+    (* solve_proper_core
+      ltac:(fun _ => first [ f_equiv | move=>?; progress cbn | rewrite iSyn_fold_unfold']). *)
+    (* solve_proper_core
+      ltac:(fun _ => first [ rewrite /= ?iSyn_fold_unfold ?iSyn_fold_unfold' | intros ?; progress simpl | f_equiv ]). *)
+  Qed.
+
+  Lemma pack_unpack Φ: pack (unpack Φ) ≡ later_pred Φ.
   Proof.
     solve_proper_core
       ltac:(fun _ => first [ rewrite iSyn_unfold_fold | intros ?; progress simpl | f_equiv ]).
@@ -83,37 +116,81 @@ Section openSemanticSyntax.
   Instance Inhabited_preD: Inhabited preD := populate (λne _ _, False)%I.
   Instance Ids_pred: Ids preD := λ _, inhabitant.
 
-  Program Definition lift_varfun {A: ofeT} (f: var → A): varC -n> A :=
-    λne x, f x.
-  Solve All Obligations with solve_proper_cbn.
+  Definition lift_varfun {A: ofeT} (f: var → A): var -c> A := f.
+  Program Definition rename_preD: (var → var) -c> preD -n> preD :=
+    λ r, λne preD ρ, preD (r >>> ρ).
+  Solve All Obligations with solve_proper_ho.
 
-  Global Program Instance Rename_preD : Rename preD :=
-    λ r preD, λne ρ, preD (lift_varfun (r >>> ρ)).
-  Solve All Obligations with solve_proper_cbn.
+  Global Instance Rename_preD : Rename preD := rename_preD.
 
-  Global Instance Rename_lpreD : Rename (laterC preD) :=
-    λ r '(Next preD), Next (rename r preD).
+  (* Global Instance Rename_lpreD : Rename (laterC preD) :=
+    λ r '(Next preD), Next (rename r preD). *)
+
   Global Instance Rename_iSyn {s}: Rename (iSyn s) := _.
+
+  Global Instance subst_prevl `{!HSubst vl preD} : Subst iPreVl :=
+    λ sb v, iSyn_unfold (subst (iSyn_fold ∘ sb) (iSyn_fold v)).
+  Global Instance subst_lprevl `{!HSubst vl preD} : Subst (laterC iPreVl) :=
+    λ sb v, iSyn_unfold' (subst (iSyn_fold' ∘ sb) (iSyn_fold' v)).
 
   Global Instance hsubst_lpreD `{!HSubst vl preD} : HSubst vl (laterC preD) :=
     λ sb '(Next preD), Next (hsubst sb preD).
-  Global Instance proper_hslpreD ρ `{!HSubst vl preD}
+
+  Global Instance syn_rename_ne {s: sort} r:
+    (* (Rename_preD0 : (var → var) → preD -n> preD):
+    let Rename_preD1 : Rename preD := (λ r v, Rename_preD0 r v) in
+    let Rename_preD : Rename (laterC preD) := (λ r '(Next v), Next (Rename_preD0 r v)) in *)
+    NonExpansive (@syn_rename preD Rename_preD s r).
+  Proof.
+    intros ** t t' Ht. move: r t' Ht.
+    induction t; intros; inversion Ht; simplify_eq; cbn; f_equiv;
+      try by [|apply IHt | apply IHt1 | apply IHt2 | f_equiv].
+  Qed.
+  (* Global Program Instance syn_up_ne: NonExpansive (@up vl _ _). *)
+  Global Instance subst_vl_preD_ne
+    (HSubstPred0 : (var -c> vl) -n> preD -n> preD):
+    let HSubstPred: HSubst vl preD := (λ sb p, HSubstPred0 sb p)
+    in NonExpansive2 (λ (s: var -c> vl), @syn_hsubst preD _ HSubstPred vls s).
+  Proof.
+    move => /= n s1 s2 Heqs x.
+    induction x => y Heq; inversion Heq; simplify_eq; cbn.
+    all: match goal with a: var, b: var, H: ?a ≡{ _ }≡ ?b |- _ => by [inversion H; apply Heqs] end || f_equiv.
+    all: rewrite /hsubst; try by [|apply IHx|apply IHx1|apply IHx2].
+    - apply IHx => //.
+      (* have Hfoo: NonExpansive (@up vl _ _). admit.
+      by eapply Hfoo. *)
+      (* Show that up is non-expansive: *)
+      rewrite // /up; move => [|i] //=. by eapply syn_rename_ne, Heqs.
+    - (* repeat f_equiv. *)
+      f_equiv => //. by apply HSubstPred0.
+  Qed.
+
+  (* Global Instance proper_hslpreD ρ `{!HSubst vl preD}
     `{proper_hspreD: ∀ ρ, NonExpansive (λ v: preD, hsubst ρ v)}:
     NonExpansive (λ v: laterC preD, hsubst ρ v).
   Proof.
     move => n [x] [y] H /=. rewrite /hsubst_lpreD.
     f_contractive. by eapply proper_hspreD.
-  Qed.
+  Qed. *)
+  (* About Subst_vl. *)
 
-  Global Instance subst_prevl `{!HSubst vl preD} : Subst iPreVl :=
-    λ sb v, iSyn_unfold (subst (λ x, (iSyn_fold (sb x))) (iSyn_fold v)).
+  (* Global Program Instance subst_vl_ne `{α: ofeT} `{Rename α} `{HSubst vl α }{s}: NonExpansive (@Subst_vl α _ _ s). *)
 
+  Program Definition hsubst_preD (rec: (var -c> vl) → preD → preD): (var -c> vl) → preD → preD :=
+    let hsubst_preD' : HSubst vl preD := rec in
+    λ sb preD, λne ρ, preD (sb >>> iSyn_unfold' >>> subst ρ).
+  Next Obligation. intros **???.
+    f_equiv=>?. rewrite /= /subst_lprevl.
+    f_equiv. rewrite /subst /Subst_vl /vl_subst /=.
+    (* The type of rec is bad. *)
+  Admitted.
+(*
   (* This will probably need some Iris fixpoint.
     And we need to lift subst to the category of OFEs. *)
-  Program Definition hsubst_preD (rec: (var → vl) → preD → preD): (var → vl) → preD → preD :=
+  Program Definition hsubst_preD (rec: (var -c> vl) → preD → preD): (var -c> vl) → preD → preD :=
     let hsubst_preD' : HSubst vl preD := rec in
-    λ sb preD, λne ρ, preD (lift_varfun (sb >>> iSyn_unfold >>> @subst _ subst_prevl ρ)).
-  Next Obligation. intros **???. f_equiv. rewrite /lift_varfun => ? /=. f_equiv. Admitted.
+    λ sb preD, λne ρ, preD (sb >>> iSyn_unfold >>> @subst _ subst_prevl ρ).
+  Next Obligation. intros **???. f_equiv. rewrite /lift_varfun => ? /=. f_equiv. Admitted. *)
 
   Global Instance discr_fun_equiv `{OfeDiscrete A} `{Equiv B} : Equiv (A → B) :=
     λ f g, ∀ x, f x ≡ g x.
@@ -142,10 +219,10 @@ Section openSemanticSyntax.
     - by intros n f g ? x; apply dist_S.
   Qed.
   Canonical Structure substC `{OfeDiscrete A} {s} : ofeT := OfeT (A → iSyn s) ofe_fun_syn_mixin.
-
-  Global Program Instance syn_rename_ne {s: sort}
+(*
+  Global Program Instance syn_rename_ne2 {s: sort}
     `{proper_hrpreD1: ∀ ρ, NonExpansive (λ v: preD, rename ρ v)}
-    `{proper_hrpreD2: NonExpansive2 (λ (ρ: varC -n> varC) (v: preD), rename ρ v)}:
+    `{proper_hrpreD2: NonExpansive2 (λ (ρ: var -c> varC) (v: preD), rename ρ v)}:
     NonExpansive2 (@syn_rename (laterC preD) _ s).
   Next Obligation.
     intros ** r1 r2 Hr t t' Ht. move: r1 r2 t' Ht Hr.
@@ -160,7 +237,7 @@ Section openSemanticSyntax.
 
   Program Definition syn_rename_ofe {s}
     `{proper_hrpreD1: ∀ ρ, NonExpansive (λ v: preD, rename ρ v)}
-    `{proper_hrpreD2: NonExpansive2 (λ (ρ: varC -n> varC) (v: preD), rename ρ v)}:
+    `{proper_hrpreD2: NonExpansive2 (λ (ρ: var -c> varC) (v: preD), rename ρ v)}:
     (varC -n> varC) -n> iSyn s -n> iSyn s :=
     λne ρ v, syn_rename ρ v.
   Solve All Obligations with solve_proper_cbn.
@@ -168,9 +245,9 @@ Section openSemanticSyntax.
 
   Program Definition syn_hsubst_ofe {s} {hspreD: HSubst vl preD}
     `{proper_hrpreD1: ∀ ρ, NonExpansive (λ v: preD, rename ρ v)}
-    `{proper_hrpreD2: NonExpansive2 (λ (ρ: varC -n> varC) (v: preD), rename ρ v)}
+    `{proper_hrpreD2: NonExpansive2 (λ (ρ: var -c> varC) (v: preD), rename ρ v)}
     `{proper_hspreD1: ∀ ρ, NonExpansive (λ v: preD, hsubst ρ v)}
-    `{proper_hspreD2: NonExpansive2 (λ (ρ: varC -n> vl) (v: preD), hsubst ρ v)}:
+    `{proper_hspreD2: NonExpansive2 (λ (ρ: var -c> vl) (v: preD), hsubst ρ v)}:
     (varC -n> vl) -n> iSyn s -n> iSyn s :=
     λne ρ v, syn_hsubst ρ v.
   Next Obligation.
@@ -215,7 +292,7 @@ Section openSemanticSyntax.
   Program Definition lift_ren {A} (r: var -> var) :=
     λne (ρ: varC -n> A),
     ofe_compose (lift_varfun r) ρ.
-  Solve All Obligations with solve_proper_cbn.
+  Solve All Obligations with solve_proper_cbn. *)
   (* ofe-variant of scomp/>>. *)
   (* Program Definition ofe_scomp {A: ofeT} {H: Subst A}
     (sb: var → A) (ρ: varC -n> A) := *)
